coq/VarList.v
@@ -1,64 +1,55 @@
 Require Import Utf8.
 Set Warnings "-notation-overridden,-parsing,-deprecated-hint-without-locality".
-From Coq Require Import Lia Bool.Bool Lists.List Strings.String Recdef Wf_nat Sorting.Permutation.
+From Coq Require Import Lia Bool.Bool Strings.String Lists.List Recdef Wf_nat Sorting.Permutation.
+From Coq Require Import ZArith.Int ZArith Lists.List.
 (* From Coq Require Import ssreflect. *)
 Require Import Coq.Classes.Equivalence.
 Import ListNotations.
 
+Require Import Syntax Utils BasicProps Algorithm PFlattenProps.
 
-Require Import Syntax Utils.
-
-Fixpoint cmp_vars (l1 l2 : var_list) : comparison :=
-  match l1, l2 with
-  | (x, n) :: l1', (y, m) :: l2' =>
-      match compare x y with
-      | Lt => Lt
-      | Gt => Gt
-      | Eq =>
-          if n <? m then Lt
-          else if m <? n then Gt
-          else cmp_vars l1' l2'
-      end
-  | [], [] => Eq
-  | _,  [] => Lt
-  | [],  _ => Gt
-  end.
-
-Lemma cmp_vars_eq_iff : ∀ v1 v2 : list (string*nat),
-  cmp_vars v1 v2 = Eq → v1 = v2.
+Lemma In_vars_dec (v : var_list) (l : list pterm) :
+  { In v (map vars l) } + {~In v (map vars l) }.
 Proof.
-  strong_list_induction.
-  intros n' IH l1 l2 Hlen Hcmp.
-  destruct l1 as [| [x n] l1'] eqn:?, l2 as [| [y m] l2'] eqn:?; auto;
-  try now inversion Hcmp.
-  simpl in Hcmp.
-  destruct (x ?= y)%string eqn:?; try discriminate.
-  pose proof (String.compare_eq_iff _ _ Heqc).
-  destruct (n <? m) eqn:?; try discriminate;
-  destruct (m <? n) eqn:?; try discriminate.
-  pose proof (nat_lt_antisym _ _ Heqb Heqb0). 
-  f_equal; [ now subst |].
-  simpl in Hlen.
-  apply (IH (len2 (l1', l2'))); auto; simpl; lia.
+  destruct In_dec with (a:=v) (l:=map vars l) as [ In | nIn ];
+  [| left; apply In
+  | right; apply nIn ].
+  apply list_eq_dec; intros [x n] [y m].
+  destruct (Nat.eq_dec n m) as [ HEqn | HnEqn ],
+           (string_dec x y) as [ HEqx | HnEqx ];
+    try (right; intro Contra; inv Contra; now auto).
+    left; f_equal; auto.
 Qed.
 
-Lemma cmp_vars_refl v : cmp_vars v v = Eq.
-Admitted.
+Lemma vars_rewrite (l1 l2 : list pterm) v :
+  l1 ≡ᵥ l2 →
+  { In v (map vars (l1++l2)) /\ cvar_count l1 v = cvar_count l2 v } +
+  { (~In v (map vars (l1++l2)) /\ cvar_count l1 v = 0 /\ cvar_count l2 v = 0)%Z }.
+Proof.
+  intros.
+  destruct (In_vars_dec v (l1++l2)).
+  - left; split;  [ assumption | apply H, i ].
+  - right; split; [ assumption |].
+    assert (∀ l, ~In v (map vars l) → cvar_count l v = 0%Z). 
+    { clear. induction l as [| [c v'] l']; simpl; intro H; auto.
+      destruct (Decidable.not_or _ _ H).
+      destruct (cmp_vars v' v) eqn:Eq; [ pose proof (cmp_vars_eq_iff _ _ Eq); exfalso; auto | |];
+      apply IHl', H1. }
+    rewrite map_app in n.
+    split; apply H0; intro H1;
+    apply n, in_or_app; [ left | right ]; apply H1.
+Qed.
 
-Fixpoint cvar_count (l : list pterm) (x : var_list) : Z :=
-  match l with
-  | PTerm c v :: l' =>
-      match cmp_vars v x with
-      | Eq => (c + cvar_count l' x)%Z
-      | _ => cvar_count l' x
-      end
-  | [] => 0
-  end.
-
-Definition vlequiv (l1 l2 : list pterm) :=
-  ∀ vars : var_list, cvar_count l1 vars = cvar_count l2 vars.
-Hint Unfold vlequiv : core.
-Notation "a '≡ᵥ' b" := (vlequiv a b) (at level 70).
+Lemma vars_nIn (v : var_list) (l : list pterm) :
+  ~In v (map vars l) →
+  cvar_count l v = 0%Z.
+Proof.
+  induction l as [| [ c v' ] l]; simpl; intros; auto.
+  destruct (Decidable.not_or _ _ H).
+  destruct (cmp_vars v' v) eqn:Eq;
+  try apply IHl, H1.
+  pose proof (cmp_vars_eq_iff _ _ Eq); exfalso; auto.
+Qed.
 
 Lemma vlequiv_app l1 l2 vars :
   cvar_count (l1++l2) vars = (cvar_count l1 vars + cvar_count l2 vars)%Z.
@@ -72,7 +63,7 @@ Lemma vlequiv_perm (la lb : list pterm) :
   Permutation la lb → vlequiv la lb.
 Proof.
   generalize dependent lb.
-  induction la as [| [c v] la']; simpl; intros lb HPerm vars; auto.
+  induction la as [| [c v] la']; simpl; intros lb HPerm vars HIn; auto.
   - pose proof (Permutation_nil HPerm); now subst.
   - symmetry in HPerm.
     pose proof (Permutation_vs_cons_inv HPerm) as [l1 [l2 Hdiv]]; subst.
@@ -81,40 +72,106 @@ Proof.
     pose proof (Permutation_cons_inv H); symmetry in H0.
     rewrite vlequiv_app; simpl.
     rewrite (IHla' _ H0).
-    rewrite vlequiv_app.
-    destruct (cmp_vars v vars); lia.
-Qed.
+    + rewrite vlequiv_app.
+      destruct (cmp_vars v vars); lia.
+    + simpl in HIn.
+Admitted.
 
 Lemma vlequiv_skip l1 : ∀ a l2,
   vlequiv l1 l2 → vlequiv (a :: l1) (a :: l2).
 Proof.
-  induction l1; simpl; intros b l2 H vars.
+  induction l1; simpl; intros b l2 H vars HIn.
   - simpl; rewrite <- H.
     destruct b as [c v], (cmp_vars v vars); simpl; lia.
+    admit.
   - remember (a::l1) as l1'.
     simpl; subst.
-    now rewrite H.
-Qed.
+    rewrite H; [ now simpl |].
+    admit.
+Admitted.
+
+Lemma cvar_count_app l1 : ∀ l2 v,
+  cvar_count (l1++l2) v = (cvar_count l1 v + cvar_count l2 v)%Z.
+Admitted.
 
 Lemma vlequiv_skip_rev l1 : ∀ a l2,
   vlequiv l1 l2 → vlequiv (a :: l1) (l2 ++ [a]).
 Proof.
-  induction l1; simpl; intros b l2 H vars.
-  - simpl. rewrite vlequiv_app, <- H. now simpl.
-  - remember (a::l1) as l1'.
-    simpl; subst.
-    destruct l2.
-    + rewrite H; simpl.
-      destruct b, (cmp_vars vars0 vars); simpl; lia.
-    + rewrite vlequiv_app, <- H; simpl.
-      destruct b, (cmp_vars vars0 vars); simpl;
-      destruct a, (cmp_vars vars1 vars); simpl; lia.
+  induction l1 as [| [c1 v1] l1]; simpl; intros b l2 H vars [Heq|HIn].
+  - destruct (vars_rewrite _ _ vars H) as [[? ?] | [? [? ?]]].
+    + simpl; rewrite vlequiv_app, <- H; auto.
+    + now rewrite vlequiv_app, H2.
+  - destruct (vars_rewrite _ _ vars H) as [[? ?] | [? [? ?]]].
+    + simpl; rewrite vlequiv_app, <- H; auto.
+    + now rewrite vlequiv_app, H2.
+  - remember (PTerm c1 v1::l1) as l1'.
+    simpl; subst vars.
+    destruct b as [c v], (vars_rewrite _ _ v H) as [[? ?] | [? [? ?]]]; f_equal; simpl.
+    + rewrite cvar_count_app, H1; simpl; rewrite cmp_vars_refl; lia.
+    + rewrite cvar_count_app, H1; simpl; rewrite cmp_vars_refl; lia.
+  - remember (PTerm c1 v1::l1) as l1'.
+    simpl.
+    destruct b as [c v], (vars_rewrite _ _ vars H) as [[? ?] | [? [? ?]]]; f_equal.
+    + rewrite H1, cvar_count_app; simpl; destruct (cmp_vars v vars); lia.
+    + rewrite H1, cvar_count_app; simpl; destruct (cmp_vars v vars); lia.
 Qed.
 
 Lemma vlequiv_list_perm (la lb : list(list pterm)) :
   Permutation la lb → vlequiv (List.concat la) (List.concat lb).
 Proof.
 Admitted.
+
+Lemma polynom_difference :
+  ∀ l1 l2, l1 ≡ₗ l2 ↔
+  [] ≡ₗ (l1 ++ map flip_sign l2).
+  (* ∀ st, 0%Z = (eval_pterm_list st l1 - eval_pterm_list st l2)%Z. *)
+Proof.
+  intros; split; intro. {
+    intro st; rewrite eval_pterm_list_homo, H; clear.
+    rewrite eval_pterm_list_map_flip; apply Zminus_diag_reverse.
+  } {
+    intro st; unfold ptequiv in *; specialize H with st.
+    rewrite eval_pterm_list_homo, eval_pterm_list_map_flip in H.
+    symmetry in H; pose proof (Zminus_eq _ _ H); auto.
+  }
+Qed.
+
+Lemma var_list_canonality_helper l1 l2 :
+  Exists (λ v : var_list, cvar_count l1 v ≠ cvar_count l2 v)
+    (map vars (l1 ++ l2)) → ~(l1 ≡ₗ l2). 
+Proof.
+  intro H; apply Exists_exists in H; destruct H as [v [HIn Hneq]].
+  intro; apply polynom_difference in H.
+Admitted.
+
+Theorem var_list_canonality :
+  ∀ l1 l2, l1 ≡ₗ l2 →
+  pterm_list_well_formed l1 → pterm_list_well_formed l2 →
+  no_zero_powers l1 → no_zero_powers l2 →
+  l1 ≡ᵥ l2.
+Proof.
+  intros l1 l2 Heqv Hwf1 Hwf2 Hnz1 Hnz2 v.
+  unfold vlequiv.
+  remember (λ v, cvar_count l1 v = cvar_count l2 v) as P.
+  replace (cvar_count l1 v = cvar_count l2 v) with (P v); [| now rewrite HeqP ].
+  generalize dependent v.
+  apply Forall_forall, not_Exists_not_Forall; subst; intro; [ apply Z.eq_dec |].
+  apply Exists_exists in H; destruct H as [v [HIn Hneq]].
+
+Abort.
+
+
+
+
+
+
+
+
+
+
+
+
+
 
 (* Reserved Notation "a '=ᵥ' b" (at level 70). *)
 (**)
