coq/Algorithm.v
@@ -1,0 +1,207 @@
+Require Import Utf8.
+From Coq Require Import ZArith.Int ZArith Lists.List.
+From Coq Require Import Lia Strings.String.
+From Coq Require Import Recdef Wf_nat.
+Require Import Syntax Utils BasicProps.
+
+Import Int.
+Open Scope Int_scope.
+Import ListNotations.
+Import List.
+
+(* ======================================================================== *)
+(* poly_flatten *)
+
+Definition flip_sign pt :=
+  match pt with
+  | PTerm c vars => PTerm (- c) vars
+  end.
+
+Function merge_vl (p : var_list*var_list) {measure len2 p} : var_list :=
+  let '(vl1, vl2) := p in
+  match vl1, vl2 with
+  | (x, n) :: vl1', (y, m) :: vl2' =>
+      if (x <? y)%string then
+        (x, n) :: merge_vl (vl1', vl2)
+      else if (y <? x)%string then
+        (y, m) :: merge_vl (vl1, vl2')
+      else (x, n+m) :: merge_vl (vl1', vl2')
+  | [], _ => vl2
+  | _, [] => vl1
+  end.
+Proof.
+  all: unfold len2; simpl; lia.
+Defined.
+Opaque merge_vl.
+
+Definition times_pterm pt1 pt2 :=
+  match pt1, pt2 with
+  | PTerm c1 vars1,
+    PTerm c2 vars2 =>
+    PTerm (c1 * c2) (merge_vl (vars1, vars2))
+  end.
+
+Fixpoint poly_flatten (a : aexp) : list pterm :=
+  match a with
+  | ANum n       => [ PTerm n []]
+  | AId  x       => [ PTerm 1 [(x, 1)]]
+  | APlus  a1 a2 => poly_flatten a1 ++ poly_flatten a2
+  | AMinus a1 a2 => poly_flatten a1 ++ map flip_sign (poly_flatten a2)
+  | AMult  a1 a2 => cross times_pterm (poly_flatten a1) (poly_flatten a2)
+  end.
+
+(* ======================================================================== *)
+(* clear_zero_powers *)
+
+Fixpoint clear_zero_powers_vl (l : var_list) : var_list :=
+  match l with
+  | (x , n) :: l' =>
+    if n =? 0
+    then clear_zero_powers_vl l'
+    else (x, n) :: clear_zero_powers_vl l'
+  | [] => []
+  end.
+
+Fixpoint clear_zero_powers (l : list pterm) : list pterm :=
+  match l with
+  | PTerm c v :: l' =>
+      PTerm c (clear_zero_powers_vl v) :: clear_zero_powers l'
+  | [] => []
+  end.
+
+(* ======================================================================== *)
+(* reduce_monom *)
+
+Function mergesort_monom (p : list pterm*list pterm) {measure len2 p} :=
+  let '(l1, l2) := p in
+  match l1, l2 with
+  | PTerm c1 v1 :: l1',
+    PTerm c2 v2 :: l2' =>
+    match cmp_vars v1 v2 with
+    | Lt => PTerm c1 v1 :: mergesort_monom (l1', l2)
+    | _ => PTerm c2 v2 :: mergesort_monom (l1, l2')
+    (* | Eq => PTerm (c1+c2) v1 :: merge_monom (l1', l2') *)
+    end
+  | [], _ => l2
+  | _, [] => l1
+  end.
+Proof.
+  all: simpl; lia.
+Defined.
+Opaque mergesort_monom.
+
+Fixpoint split {X:Type} (l:list X) : (list X * list X) :=
+  match l with
+  | [] => ([],[])
+  | [x] => ([x],[])
+  | x1::x2::l' =>
+    let (l1,l2) := split l' in
+    (x1::l1,x2::l2)
+  end.
+
+Lemma split_len:
+    forall {X} (l:list X) (l1 l2: list X),
+    split l = (l1,l2) ->
+    List.length l1 <= List.length l /\
+    List.length l2 <= List.length l.
+Proof.
+  assert (IP: forall (A : Type) (P : list A -> Prop),
+      P [] ->
+      (forall (a:A), P [a]) ->
+      (forall (a b : A) (l : list A), P l -> P (a :: b :: l)) ->
+      forall l : list A, P l)
+  by refine (fun (A : Type)
+      (P : list A -> Prop)
+      (H : P [])
+      (H0 : forall a : A, P [a])
+      (H1 : forall (a b : A) (l : list A), P l -> P (a :: b :: l))  =>
+    fix IH (l : list A) :  P l :=
+    match l with
+    | [] => H
+    | [x] => H0 x
+    | x::y::l' => H1 x y l' (IH l')
+    end).
+  induction l using IP; intros.
+  - inv H. lia.
+  - inv H. simpl; lia.
+  - inv H. destruct (split l) as [l1' l2']. inv H1.
+    simpl.
+    destruct (IHl l1' l2') as [P1 P2]; auto; lia.
+Qed.
+
+Function sort_monomials (l : list pterm) {measure List.length l} :=
+  match l with
+  | [] => []
+  | [x] => [x]
+  | _ => 
+    let '(l1, l2) := split l in
+    mergesort_monom (sort_monomials l1, sort_monomials l2)
+  end.
+Proof.
+  - intros.
+    simpl in *. destruct (split l1) as [l1' l2'] eqn:E. inv teq1. simpl.
+    destruct (split_len _ _ _ E).
+    lia.
+  - intros.
+    simpl in *. destruct (split l1) as [l1' l2'] eqn:E. inv teq1. simpl.
+    destruct (split_len _ _ _ E).
+    lia.
+Defined.
+
+Function reduce_monomials (l : list pterm) {measure List.length l} :=
+  match l with
+  | [] => []
+  | [PTerm c v] =>
+    if (c =? 0)%Z
+    then []
+    else [PTerm c v]
+  | PTerm c1 v1 :: (PTerm c2 v2 :: l') as l =>
+    match cmp_vars v1 v2 with
+    | Eq => reduce_monomials (PTerm (c1+c2) v1 :: l')
+    | _  =>
+      if (c1 =? 0)%Z
+      then reduce_monomials l
+      else PTerm c1 v1 :: reduce_monomials l
+    end
+  end.
+Proof.
+  all: intros; simpl; lia.
+Defined.
+
+
+(* ======================================================================== *)
+(* poly_simpl *)
+
+Fixpoint reconstruct_var_pow x n :=
+  match n with
+  | 0    => ANum 1
+  | S 0  => AId x
+  | S n' => AMult (AId x) (reconstruct_var_pow x n')
+  end.
+
+Fixpoint reconstruct_monom c (l : var_list) : aexp :=
+  match l with
+  | [] => ANum c
+  | (x, n) :: l' =>
+      AMult (reconstruct_var_pow x n) (reconstruct_monom c l')
+  end.
+
+Fixpoint reconstruct (l : list pterm) : aexp :=
+  match l with
+  | [] => ANum 0
+  | [PTerm c vars] => reconstruct_monom c vars
+  | PTerm c vars :: l' =>
+      APlus (reconstruct_monom c vars) (reconstruct l')
+  end.
+
+(* ======================================================================== *)
+(* poly_simpl *)
+
+Definition poly_simpl (a : aexp) :=
+  let l1 := poly_flatten a in
+  let l2 := clear_zero_powers l1 in
+  let l3 := sort_monomials l2 in
+  let l4 := reduce_monomials l3 in
+  reconstruct l4.
+
+
