coq/BasicProps.v
@@ -1,0 +1,204 @@
+Require Import Utf8.
+From Coq Require Import ZArith.Int ZArith Lists.List Sorting.Sorted.
+Require Import Syntax.
+
+Import Int.
+Import ListNotations.
+
+(* ======================================================================== *)
+(* Evaluation equivalence properties *)
+
+Inductive pterm :=
+  | PTerm (c : Z) (vars : var_list).
+
+Definition vars '(PTerm _ vars) := vars.
+Definition const '(PTerm c _) := c.
+
+Definition pow (st : state) '(x, n) : Z :=
+  Z.pow (st x) (Z.of_nat n).
+
+Definition eval_pterm (st : state) '(PTerm c vars) : Z :=
+  fold_left Z.mul (map (pow st) vars) c.
+
+Fixpoint eval_pterm_list (st : state) (l : list pterm) : Z :=
+  match l with
+  | [] => 0_
+  | c :: l' => eval_pterm_list st l' + eval_pterm st c
+  end.
+
+Definition aequiv (a1 a2 : aexp) : Prop :=
+  forall (st : state),
+    aeval st a1 = aeval st a2.
+Hint Unfold aequiv : core.
+
+Notation "a '≡' b" :=  (aequiv a b) (at level 70).
+
+Definition ptequiv (l1 l2 : list pterm) : Prop :=
+  forall (st : state),
+    eval_pterm_list st l1 = eval_pterm_list st l2.
+Hint Unfold ptequiv : core.
+
+Notation "a '≡ₗ' b" :=  (ptequiv a b) (at level 70).
+
+Definition asimpt a l :=
+  forall st : state, aeval st a = eval_pterm_list st l.
+Hint Unfold asimpt : core.
+
+Notation "a '≲ₗ' l" := (asimpt a l) (at level 70).
+
+(* ======================================================================== *)
+(* Main Properties *)
+
+Definition Correctness (f : aexp → aexp) :=
+  forall a : aexp, a ≡ f a.
+Hint Unfold Correctness : core.
+
+Definition Canonality (f : aexp → aexp) :=
+  forall a1 a2, a1 ≡ a2 → f a1 = f a2.
+Hint Unfold Canonality : core.
+
+(* ======================================================================== *)
+(* basic pterm properties *)
+
+Inductive sorted_uniq : list (string*nat) -> Prop :=
+| sorted_nil:
+    sorted_uniq []
+| sorted_1: forall x,
+    sorted_uniq [x]
+| sorted_cons: forall x y l,
+    (fst x <? fst y)%string = true ->
+    sorted_uniq (y :: l) ->
+    sorted_uniq (x :: y :: l).
+Hint Constructors sorted_uniq : core.
+
+Definition pterm_list_well_formed (l : list pterm) :=
+  Forall (λ '(PTerm _ vars), sorted_uniq vars) l.
+Hint Unfold pterm_list_well_formed : core.
+
+Definition no_zero_powers (l : list pterm) :=
+  Forall (λ '(PTerm _ vars),
+    Forall (λ '(_, n), n <> 0) vars) l.
+Hint Unfold no_zero_powers : core.
+
+(* ======================================================================== *)
+(* grouped pterm properties *)
+
+Fixpoint grouped_eval_pl (st : state) (l : list (list pterm)) :=
+  match l with
+  | [] => 0%Z
+  | ls :: l' => (eval_pterm_list st ls + grouped_eval_pl st l')%Z
+  end.
+
+Definition grouped_eval_equiv l1 l2 :=
+  ∀ st, grouped_eval_pl st l1 = grouped_eval_pl st l2. 
+Hint Unfold grouped_eval_equiv : core.
+Notation "a '≡ₚ' b" := (grouped_eval_equiv a b) (at level 70).
+
+Definition pterm_equiv (p1 p2 : pterm) :=
+  let '(PTerm _ v1) := p1 in
+  let '(PTerm _ v2) := p2 in
+  v1 = v2.
+
+Inductive equiv_list : list pterm → Prop :=
+  | EL_Single a :
+      equiv_list [a]
+  | EL_Cons a b l :
+      equiv_list (a :: l) →
+      pterm_equiv a b →
+      equiv_list (b :: a :: l).
+Hint Constructors equiv_list : core.
+
+Inductive Disjoint : list (list pterm) → Prop :=
+  | disjoint_nil : Disjoint []
+  | disjoint_single l :
+      equiv_list l →
+      Disjoint [l]
+  | disjoint_cons p p' (l l' : list pterm) (ls : list (list pterm)) :
+      equiv_list (p::l) →
+      ~In (p'::l') ls →
+      pterm_equiv p p' →
+      Disjoint ls →
+      Disjoint ((p::l)::ls).
+Hint Constructors Disjoint : core.
+
+Definition grouped_pterms (l : list (list pterm)) :=
+  Forall equiv_list l /\ Disjoint l.
+Hint Unfold grouped_pterms : core.
+
+(* ======================================================================== *)
+(* variables equivalence properties *)
+
+Fixpoint cmp_vars (l1 l2 : var_list) : comparison :=
+  match l1, l2 with
+  | (x, n) :: l1', (y, m) :: l2' =>
+      match compare x y with
+      | Lt => Lt
+      | Gt => Gt
+      | Eq =>
+          if n <? m then Lt
+          else if m <? n then Gt
+          else cmp_vars l1' l2'
+      end
+  | [], [] => Eq
+  | _,  [] => Lt
+  | [],  _ => Gt
+  end.
+
+Fixpoint cvar_count (l : list pterm) (x : var_list) : Z :=
+  match l with
+  | PTerm c v :: l' =>
+      match cmp_vars v x with
+      | Eq => (c + cvar_count l' x)%Z
+      | _ => cvar_count l' x
+      end
+  | [] => 0
+  end.
+
+Definition vlequiv (l1 l2 : list pterm) :=
+  ∀ v : var_list, In v (map vars (l1 ++ l2)) →
+    cvar_count l1 v = cvar_count l2 v.
+Hint Unfold vlequiv : core.
+Notation "a '≡ᵥ' b" := (vlequiv a b) (at level 70).
+
+(* ======================================================================== *)
+(* grouped pterm properties *)
+
+Inductive grouped_flat : list pterm → Prop :=
+  | GF_nil : grouped_flat []
+  | GF_single l :
+      grouped_flat [l]
+  | GF_last_rep p p' l :
+      ~In p' l →
+      pterm_equiv p p' →
+      grouped_flat l →
+      grouped_flat (p :: l)
+  | GF_cons p p' l :
+      pterm_equiv p p' →
+      grouped_flat (p' :: l) →
+      grouped_flat (p :: p' :: l)
+  .
+Hint Constructors grouped_flat : core.
+
+Inductive canon_pterm : list pterm → Prop :=
+  | CP_nil : canon_pterm []
+  | CP_cons p p' l :
+      ~In p' l →
+      pterm_equiv p p' →
+      canon_pterm l →
+      canon_pterm (p :: l)
+  .
+Hint Constructors canon_pterm : core.
+
+Definition non_zero_const (ls : list pterm) :=
+  Forall (λ '(PTerm c _), c <> 0%Z) ls.
+Hint Unfold non_zero_const : core.
+
+(* ======================================================================== *)
+(* sorted pterm properties *)
+
+Definition pterm_le p1 p2 :=
+  cmp_vars (vars p1) (vars p2) <> Gt.
+Hint Unfold pterm_le : core.
+
+Definition sorted := LocallySorted pterm_le.
+Hint Unfold sorted : core.
