coq/CanonPTProps.v
@@ -1,0 +1,10 @@
+Require Import Utf8.
+Set Warnings "-notation-overridden,-parsing,-deprecated-hint-without-locality".
+From Coq Require Import Lia Strings.String Recdef Wf_nat Sorting.Permutation.
+From Coq.Lists Require Import List ListDec.
+Require Import Coq.Classes.Equivalence.
+Import ListNotations.
+
+From PolySimpl Require Import Syntax Utils VarList BasicProps.
+From PolySimpl Require Import PFlattenProps ClearZPProps ReduceMonomProps.
+
