coq/PolySimplProps.v
@@ -1,0 +1,243 @@
+Require Import Utf8.
+Set Warnings "-notation-overridden,-parsing,-deprecated-hint-without-locality".
+From Coq Require Import Lia Strings.String Recdef Wf_nat Sorting.Permutation.
+From Coq.Lists Require Import List ListDec.
+Require Import Coq.Classes.Equivalence.
+Import ListNotations.
+
+From PolySimpl Require Import Syntax Utils VarList Algorithm BasicProps.
+From PolySimpl Require Import PFlattenProps ClearZPProps ReduceMonomProps ReconstructProps.
+From Poly
+
+
+
+
+
+
+
+
+    
+
+
+
+Theorem poly_simpl_correctness : Correctness poly_simpl.
+Proof.
+  unfold Correctness, poly_simpl.
+  intros a st.
+  rewrite reconstruct_correct.
+  rewrite <- reduce_monomials_correct.
+  rewrite <- sort_monomials_correct.
+  rewrite <- clear_zero_powers_correct.
+  now rewrite <- poly_flatten_correct.
+Qed.
+
+Theorem poly_simpl_canonility : Canonality poly_simpl.
+Proof.
+  unfold Canonality, poly_simpl.
+  intros a1 a2 Heqv. f_equal.
+  apply reconstruct_canonality.
+  apply to_reduce_poly_canonality, Heqv.
+Qed.
+
+
+Lemma grouping_lemma :
+  ∀ l1 l2,
+  Forall pterm_list_well_formed l1 →
+  Forall pterm_list_well_formed l2 →
+  Forall no_zero_powers l1 →
+  Forall no_zero_powers l2 →
+  grouped_pterms l1 →
+  grouped_pterms l2 →
+  (∀ st, grouped_eval_pl st l1 = grouped_eval_pl st l2) →
+  List.concat l1 ≡ᵥ List.concat l2. 
+Proof.
+Admitted.
+
+
+Lemma reduce_monom_List_concat_homo l ls :
+  grouped_pterms (l::ls) →
+  Forall pterm_list_well_formed (l::ls) →
+  Forall no_zero_powers (l::ls) →
+  reduce_monomials (List.concat (l::ls)) =
+  reduce_monomials l ++ reduce_monomials (List.concat ls).
+Proof.
+Admitted.
+
+Lemma reduce_monom_perm_invariant :
+  ∀ l1 l2, Permutation l1 l2 →
+  pterm_list_well_formed l1 → pterm_list_well_formed l2 →
+  no_zero_powers l1 → no_zero_powers l2 →
+  reduce_monomials l1 = reduce_monomials l2.
+Proof.
+Admitted.
+
+Lemma reduce_monom_perm_invariant' :
+  ∀ l1 l2, Permutation (reduce_monomials l1) l2 →
+  reduce_monomials l1 = reduce_monomials l2.
+Proof.
+  strong_list_induction.
+  intros n' IH l1 l2 Hlen HPerm.
+  destruct l1 as [| [c1 v1] l1'] eqn:Eql1;
+  destruct l2 as [| [c2 v2] l2'] eqn:Eql2; auto;
+  (* - rewrite reduce_monomials_equation in HPerm. *)
+  [ destruct (reduce_monomials (PTerm c2 v2 :: l2')) eqn:?; auto;
+    apply Permutation_nil_cons in HPerm; contradiction
+  | destruct (reduce_monomials (PTerm c1 v1 :: l1')) eqn:?; auto;
+    symmetry in HPerm; apply Permutation_nil_cons in HPerm; contradiction |].
+  rewrite <- Eql1 in *.
+  clear Eql1 l1' c1 v1.
+  destruct (Permutation_vs_cons_inv HPerm) as [la [lb Hab]].
+  (* rewrite Hab in HP. *)
+  specialize HPerm as HPerm'; rewrite Hab in HPerm'.
+  assert (Permutation (la ++ lb) l2')
+    by (eapply Permutation_cons_inv; etransitivity; [| apply HPerm' ];
+      apply Permutation_middle).
+Abort.
+
+Lemma reduce_monomials_sorts :
+  ∀ l1 l2, Permutation l1 l2 →
+  reduce_monomials l1 = reduce_monomials l2.
+Proof.
+  strong_list1_induction.
+  intros n' IH [| [c1 v1] l1] HLen [| [c2 v2] l2] HPerm; auto.
+  - apply Permutation_nil_cons in HPerm; contradiction.
+  - symmetry in HPerm; apply Permutation_nil_cons in HPerm; contradiction.
+  - {
+  destruct l1 as [| [c1' v1'] l1'] eqn:Eql1;
+  destruct l2 as [| [c2' v2'] l2'] eqn:Eql2; auto;
+  try (apply Permutation_length in HPerm; discriminate HPerm);
+  [ apply Permutation_length_1 in HPerm; inv HPerm; subst; auto |].
+  rewrite reduce_monomials_equation; symmetry;
+  rewrite reduce_monomials_equation; symmetry.
+  destruct (split (PTerm c1 v1 :: _)) eqn:?.
+  destruct (split (PTerm c2 v2 :: _)) eqn:?.
+Abort.
+
+Theorem reduce_monomials_canonality :
+  ∀ l1 l2, l1 ≡ᵥ l2 →
+  pterm_list_well_formed l1 → pterm_list_well_formed l2 →
+  no_zero_powers l1 → no_zero_powers l2 →
+  reduce_monomials l1 = reduce_monomials l2.
+Proof.
+  strong_list_induction.
+  intros n' IH l1 l2 Hlen Heqv Hwf1 Hwf2 Hnz1 Hnz2.
+  destruct l1 as [| [c1 v1] l1'] eqn:Eql1,
+           l2 as [| [c2 v2] l2'] eqn:Eql2; auto.
+  + rewrite reduce_monomials_equation.
+Admitted.
+
+Definition rep (l : list pterm) (H: equiv_list l) : pterm.
+Proof.
+  destruct l.
+  - exfalso. inversion H.
+  - apply p.
+Defined.
+
+Fixpoint reduce_vequiv (l : list pterm) (H: equiv_list l) :
+  { p : pterm | pterm_equiv p (rep l H)}.
+Proof.
+  destruct l as [| [c1 v1] [| [c2 v2] l]];
+  [ exfalso; inv H | exists (PTerm c1 v1); now simpl |].
+  assert (equiv_list (PTerm c2 v2 :: l)) by (inv H; auto).
+  destruct (reduce_vequiv (PTerm c2 v2 :: l) H0) as [[c_res v_res] Hp].
+  simpl in Hp.
+  exists (PTerm (c1+c_res) v1); now simpl.
+Defined.
+
+Lemma reduce_vequiv_correct (l : list pterm) (H: equiv_list l) :
+  let '(PTerm c _) := proj1_sig (reduce_vequiv l H) in
+  (fold_left (λ c '(PTerm c' _), c+c') l 0)%Z = c.
+Admitted.
+
+Fixpoint reduce_grouped_monomials (ls : list (list pterm)) :
+  Forall equiv_list ls → list pterm.
+Proof.
+  intro HFa.
+  destruct ls as [| l ls]; [ apply [] |].
+  refine (let (Heqv, HFa') := (_ : equiv_list l * Forall equiv_list ls) in
+          let p := proj1_sig (reduce_vequiv l Heqv) in
+          let l := reduce_grouped_monomials ls HFa' in
+          p :: l).
+  inversion HFa; split; auto.
+Defined.
+
+Definition reduce_monomials_simply (l : list pterm) : list pterm :=
+  match group_pterms l with
+  | exist _ ls (conj (conj H _) _) =>
+      reduce_grouped_monomials ls H
+  end.
+
+Theorem merge_monom_reduce_monomials_simply : ∀ (l' l1 l2 : list pterm),
+  (* split l' = (l1, l2) → *)
+  Permutation l' (l1++l2) →
+  merge_monom (reduce_monomials_simply l1, reduce_monomials_simply l2) =
+  reduce_monomials_simply l'.
+Proof.
+  strong_list1_induction.
+  intros n' IH l' Hlen l1 l2 Hperm.
+  rewrite merge_monom_equation.
+Abort.
+
+
+Theorem reduce_monomials_spec :
+  ∀ l, Permutation (reduce_monomials l) (reduce_monomials_simply l).
+Proof.
+  strong_list_induction.
+  intros n' IH l Hlen.
+  destruct l as [| [c1 v1] [| [c2 v2] l']] eqn:?;
+      try (rewrite reduce_monomials_equation; simpl; now auto).
+  remember (PTerm c1 v1 :: PTerm c2 v2 :: l').
+  rewrite reduce_monomials_equation, Heql1.
+  destruct (split (PTerm c1 v1 :: PTerm c2 v2 :: l')) eqn:Hsplt.
+  pose proof (split_len_strict _ _ _ _ _ Hsplt) as [? ?].
+  (* rewrite (IH (List.length l1)); *)
+  (* subst; simpl in *; try lia. *)
+  (* rewrite (IH (List.length l2)); *)
+  subst; simpl in *; try lia.
+  destruct (split l') eqn:?.
+  inv Hsplt.
+  rewrite merge_monom_equation.
+  destruct (reduce_monomials _) as [| [c1' v1'] l1'] eqn:Heql1',
+           (reduce_monomials (PTerm c2 v2 :: l0)) as [| [c2' v2'] l2'] eqn:Heql2';
+  try (pose proof (reduce_monom_cons_nil _ _ Heql2'); contradiction);
+  try (pose proof (reduce_monom_cons_nil _ _ Heql1'); contradiction).
+  destruct (cmp_vars v1' v2').
+  - unfold reduce_monomials_simply.
+    destruct (group_pterms _) as [ls [[HFa Hdis] HPerm]].
+Abort.
+
+
+Theorem to_reduce_poly_canonality :
+  ∀ a1 a2, a1 ≡ a2 →
+  reduce_monomials (clear_zero_powers (poly_flatten a1)) =
+  reduce_monomials (clear_zero_powers (poly_flatten a2)).
+Proof.
+  intros a1 a2 Heqv.
+  (* Prepare some properties *)
+  assert (no_zero_powers (clear_zero_powers (poly_flatten a1)));
+  [ apply clear_zero_powers_no_zeros, poly_flatten_well_formed |].
+  assert (pterm_list_well_formed (clear_zero_powers (poly_flatten a1)));
+  [ apply clear_zero_powers_well_formed_preserving,
+          poly_flatten_well_formed |].
+  assert (no_zero_powers (clear_zero_powers (poly_flatten a2)));
+  [ apply clear_zero_powers_no_zeros, poly_flatten_well_formed |].
+  assert (pterm_list_well_formed (clear_zero_powers (poly_flatten a2)));
+  [ apply clear_zero_powers_well_formed_preserving,
+          poly_flatten_well_formed |].
+  (* reduce_monomials produces unique pterm lists *)
+  apply reduce_monomials_canonality; auto.
+  apply var_list_canonality; auto.
+  intro st.
+  repeat rewrite <- clear_zero_powers_correct.
+  now repeat rewrite <- poly_flatten_correct.
+Qed.
+
+Theorem reconstruct_canonality :
+  ∀ l1 l2, l1 = l2 →
+  reconstruct l1 = reconstruct l2.
+Proof.
+  induction l1; simpl; intros l2 Heq;
+  now rewrite <- Heq.
+Qed.
+
+
