coq/PolyUniqueness.v
@@ -1,0 +1,17 @@
+Require Import Utf8.
+Set Warnings "-notation-overridden,-parsing,-deprecated-hint-without-locality".
+From Coq Require Import Lia Lists.List Strings.String Recdef Wf_nat Sorting.Sorted.
+Import ListNotations.
+
+From PolySimpl Require Import Syntax Utils BasicProps Algorithm VarList.
+
+Theorem polynom_uniqueness :
+  ∀ l1 l2, l1 ≡ₗ l2 →
+  sorted l1 → sorted l2 →
+  canon_pterm l1 → canon_pterm l2 →
+  non_zero_const l1 → non_zero_const l2 →
+  l1 = l2.
+Proof.
+  strong_list_induction.
+  intros n' IH l1 l2 Hlen Heqv Hsort1 Hsort2 Hcanon1 Hcanon2 Hnzc1 Hnzc2.
+Admitted.
