coq/ReduceMonomProps.v
@@ -1,24 +1,22 @@
 Require Import Utf8.
 Set Warnings "-notation-overridden,-parsing,-deprecated-hint-without-locality".
-From Coq Require Import Lia Lists.List Strings.String Recdef Wf_nat.
+From Coq Require Import Lia Recdef Wf_nat.
+From Coq Require Import Bool.Bool Lists.List Strings.String Sorting.Sorted.
 Import ListNotations.
 
-From PolySimpl Require Import Syntax Utils ClearZP ReduceMonom VarList.
+From PolySimpl Require Import Syntax Utils BasicProps Algorithm VarList.
 
 Lemma merge_monom_correct (st : state) :
   ∀ l1 l2,
   (eval_pterm_list st l1 + eval_pterm_list st l2)%Z =
-    eval_pterm_list st (merge_monom (l1, l2)).
+    eval_pterm_list st (mergesort_monom (l1, l2)).
 Proof.
   strong_list_induction.
   intros n IH [| [c1 v1] l1] [| [c2 v2] l2] Hlen;
-  rewrite merge_monom_equation; auto using Z.add_0_r.
+  rewrite mergesort_monom_equation; auto using Z.add_0_r.
   destruct (cmp_vars v1 v2) eqn:?; simpl in *.
   - pose proof (cmp_vars_eq_iff _ _ Heqc); subst.
-    rewrite <- (IH (len2 (l1, l2))); simpl; try lia.
-    repeat rewrite <- Z.add_assoc.
-    f_equal.
-    now rewrite Z.add_comm, <- Z.add_assoc, fold_left_mul_add_distr.
+    rewrite <- (IH (1+len2 (l1, l2))); simpl; try lia.
   - rewrite <- (IH (1+len2(l1, l2))); simpl; lia.
   - rewrite <- (IH (1+len2(l1, l2))); simpl; lia.
 Qed.
@@ -42,7 +40,7 @@ Lemma split_eval_pt_correct :
   ∀ st, eval_pterm_list st l =
   (eval_pterm_list st l1 + eval_pterm_list st l2)%Z.
 Proof.
-  strong_list1_induction.
+strong_list1_induction.
   intros n IH l Hlen l1 l2 Hsplit st.
   destruct l as [| [c1 v1] [| [c2 v2] l']] eqn:?;
   try now (inv Hsplit; auto using Z.add_0_r).
@@ -96,16 +94,16 @@ Lemma merge_monom_wf_preserving :
   ∀ l1 l2,
   pterm_list_well_formed l1 →
   pterm_list_well_formed l2 →
-  pterm_list_well_formed (merge_monom (l1, l2)).
+  pterm_list_well_formed (mergesort_monom (l1, l2)).
 Proof.
   strong_list_induction.
   intros n' IH l1 l2 Hlen Hnz1 Hnz2.
-  rewrite merge_monom_equation.
+  rewrite mergesort_monom_equation.
   destruct l1 as [| [c1 v1] l1'] eqn:Eql1,
            l2 as [| [c2 v2] l2'] eqn:Eql2; auto.
   destruct (cmp_vars v1 v2) eqn:?.
   - inversion Hnz1; inversion Hnz2; constructor; auto.
-    apply (IH (len2 (l1', l2'))); simpl in *; subst; auto; lia.
+    apply (IH (1+len2 (l1', l2'))); simpl in *; subst; auto; lia.
   - inversion Hnz1; inversion Hnz2; constructor; auto.
     apply (IH (1+len2 (l1', l2'))); simpl in *; subst; auto; lia.
   - inversion Hnz1; inversion Hnz2; constructor; auto.
@@ -116,28 +114,127 @@ Lemma merge_monom_nz_preserving :
   ∀ l1 l2,
   no_zero_powers l1 →
   no_zero_powers l2 →
-  no_zero_powers (merge_monom (l1, l2)).
+  no_zero_powers (mergesort_monom (l1, l2)).
 Proof.
   strong_list_induction.
   intros n' IH l1 l2 Hlen Hnz1 Hnz2.
-  rewrite merge_monom_equation.
+  rewrite mergesort_monom_equation.
   destruct l1 as [| [c1 v1] l1'] eqn:Eql1,
            l2 as [| [c2 v2] l2'] eqn:Eql2; auto.
   destruct (cmp_vars v1 v2) eqn:?.
   - inversion Hnz1; inversion Hnz2; constructor; auto.
-    apply (IH (len2 (l1', l2'))); simpl in *; subst; auto; lia.
+    apply (IH (1+len2 (l1', l2'))); simpl in *; subst; auto; lia.
   - inversion Hnz1; inversion Hnz2; constructor; auto.
     apply (IH (1+len2 (l1', l2'))); simpl in *; subst; auto; lia.
   - inversion Hnz1; inversion Hnz2; constructor; auto.
     apply (IH (1+len2 (l1', l2'))); simpl in *; subst; auto; lia.
 Qed.
 
-Theorem reduce_monomials_correct :
-  ∀ l, l ≡ₗ (reduce_monomials l).
+Lemma mergesort_monomials_sorted1 : forall x x1 l1 x2 l2,
+    pterm_le x x1 -> pterm_le x x2 ->
+    sorted (mergesort_monom (x1::l1, x2::l2)) ->
+    sorted (x :: mergesort_monom (x1::l1, x2::l2)).
+Proof.
+  intros.
+  rewrite mergesort_monom_equation in *.
+  destruct x1 as [c1 v1], x2 as [c2 v2].
+  destruct (cmp_vars v1 v2);
+  constructor; assumption.
+Qed.
+
+Lemma mergesort_monomials_sorted : forall l1, sorted l1 ->
+                     forall l2, sorted l2 ->
+                     sorted (mergesort_monom (l1, l2)).
+Proof.
+  induction l1 as [| [c1 v1] l1]; intros;
+  [ simpl; destruct l2; auto |].
+  induction l2 as [| [c2 v2] l2]; rewrite mergesort_monom_equation; auto.
+  cbn.
+  enough (cmp_vars v1 v2 = Lt → sorted (PTerm c1 v1 :: mergesort_monom (l1, PTerm c2 v2 :: l2)));
+  [ enough (cmp_vars v1 v2 <> Lt → sorted (PTerm c2 v2 :: mergesort_monom (PTerm c1 v1 :: l1, l2))) |];
+  [ (destruct (cmp_vars v1 v2); auto); apply H2; intro HC; discriminate | |]; intro HLt.
+  - assert (∀ v1 v2, cmp_vars v1 v2 <> Lt → cmp_vars v2 v1 <> Gt). {
+      clear; intros v1 v2 HLt.
+      intro C. apply HLt. rewrite cmp_vars_antisym.
+      unfold CompOpp. now rewrite C. }
+    destruct l2 as [| [c2' v2'] l2];
+    [ constructor; unfold pterm_le; auto |].
+    inv H0; unfold pterm_le in *; simpl in *.
+    apply mergesort_monomials_sorted1; unfold pterm_le; auto; simpl.
+  - assert (∀ v1 v2, cmp_vars v1 v2 = Lt → cmp_vars v1 v2 <> Gt). {
+      clear; simpl; intros v1 v2 HLt HGt.
+      rewrite HGt in HLt; discriminate. }
+    destruct l1 as [| [c1' v1'] l1];
+    [ constructor; unfold pterm_le; auto |].
+    inv H; unfold pterm_le in *; simpl in *.
+    apply mergesort_monomials_sorted1; unfold pterm_le; auto; simpl.
+Qed.
+
+Lemma vars_pow_add v c1 c2 st :
+  (fold_left Z.mul (map (pow st) v) c2 + fold_left Z.mul (map (pow st) v) c1)%Z =
+  fold_left Z.mul (map (pow st) v) (c1 + c2)%Z.
+Proof.
+  induction v; simpl; try lia.
+  repeat rewrite <- fold_left_mul_acc.
+  now rewrite <- Z.mul_add_distr_r, <- IHv.
+Qed.
+
+Lemma HdRel_pterm_le_const_invariant c1 c2 v l :
+  HdRel pterm_le (PTerm c2 v) l →
+  HdRel pterm_le (PTerm c1 v) l.
+Proof.
+  induction l; auto.
+  intros H. inv H.
+  econstructor; apply H1.
+Qed.
+
+Lemma reduce_monomials_HdRel_pterm_le :
+  ∀ l c1 c2 v1 v2,
+  cmp_vars v1 v2 = Lt →
+  sorted (PTerm c1 v1 :: PTerm c2 v2 :: l) →
+  HdRel pterm_le (PTerm c1 v1) (reduce_monomials (PTerm c2 v2 :: l)).
+Proof.
+  strong_list_induction.
+  intros n' IH l Hlen c1 c2 v1 v2 Hcmp Hsort.
+  destruct l as [| [c3 v3] l'] eqn:?; auto;
+  rewrite reduce_monomials_equation.
+  { destruct (Z.eqb_spec c2 0); auto.
+    constructor. unfold pterm_le; simpl.
+    intro H; rewrite H in Hcmp; discriminate. }
+  destruct (cmp_vars v2 v3) eqn:?.
+  - simpl in *.
+    apply (IH (List.length l')); try (subst; simpl; lia); auto.
+    pose proof (cmp_vars_eq_iff _ _ Heqc); subst v3.
+    apply Sorted_LocallySorted_iff.
+    apply Sorted_LocallySorted_iff in Hsort.
+    inv Hsort. inv H1. inv H3.
+    econstructor.
+    + econstructor; auto.
+      eapply HdRel_pterm_le_const_invariant, H5.
+    + inv H2.
+      econstructor; unfold pterm_le in *; now simpl in *.
+  - destruct (Z.eqb_spec c2 0).
+    + apply Sorted_LocallySorted_iff, Sorted_StronglySorted in Hsort;
+        [| apply Rel1_Transitive_pterm_le ].
+      inversion Hsort; inversion H1.
+      assert (StronglySorted pterm_le (PTerm c1 v1 :: PTerm c3 v3 :: l'))
+        by (inv H2; econstructor; auto).
+      simpl in Hlen; apply StronglySorted_Sorted, Sorted_LocallySorted_iff in H7;
+      apply (IH (List.length l')); try (subst; simpl; lia); auto.
+      eapply cmp_vars_trans; eauto.
+    + econstructor.
+      unfold pterm_le in *; simpl in *.
+      intro HGt; rewrite HGt in Hcmp; discriminate.
+  - inv Hsort. inv H1. unfold pterm_le in H5; simpl in H5.
+    exfalso; apply H5, Heqc.
+Qed.
+
+Theorem sort_monomials_correct :
+  ∀ l, l ≡ₗ (sort_monomials l).
 Proof.
   strong_list_induction.
   intros n IH [| [c1 v1] [| [c2 v2] l]] Hlen st;
-  rewrite reduce_monomials_equation; auto.
+  rewrite sort_monomials_equation; auto.
   destruct (split (PTerm c1 v1 :: PTerm c2 v2 :: l)) eqn:?.
   specialize (split_len_strict  _ _ _ _ _ Heqp) as [Hlen0 Hlen1]; 
   rewrite <- merge_monom_correct; simpl.
@@ -151,12 +248,12 @@ Proof.
   lia.
 Qed.
 
-Theorem reduce_monomials_well_formed_preserving : ∀ l : list pterm,
+Theorem sort_monomials_well_formed_preserving : ∀ l : list pterm,
   pterm_list_well_formed l →
-  pterm_list_well_formed (reduce_monomials l).
+  pterm_list_well_formed (sort_monomials l).
 Proof.
   strong_list_induction.
-  intros n IH l Hlen Hwf; rewrite reduce_monomials_equation.
+  intros n IH l Hlen Hwf; rewrite sort_monomials_equation.
   destruct l as [| [c1 ?] [| [c2 ?] l']] eqn:?; auto.
   destruct (split (PTerm c1 vars :: PTerm c2 vars0 :: l')) eqn:?.
   specialize (split_len_strict _ _ _ _ _ Heqp) as [? ?].
@@ -174,12 +271,12 @@ Proof.
     now apply Forall_forall.
 Qed.
 
-Theorem reduce_monomials_no_zeros_preserving : ∀ l : list pterm,
+Theorem sort_monomials_no_zeros_preserving : ∀ l : list pterm,
   no_zero_powers l →
-  no_zero_powers (reduce_monomials l).
+  no_zero_powers (sort_monomials l).
 Proof.
   strong_list_induction.
-  intros n IH l Hlen Hwf; rewrite reduce_monomials_equation.
+  intros n IH l Hlen Hwf; rewrite sort_monomials_equation.
   destruct l as [| [c1 ?] [| [c2 ?] l']] eqn:?; auto.
   destruct (split (PTerm c1 vars :: PTerm c2 vars0 :: l')) eqn:?.
   specialize (split_len_strict _ _ _ _ _ Heqp) as [? ?].
@@ -197,4 +294,226 @@ Proof.
     now apply Forall_forall.
 Qed.
 
+Theorem sort_monomials_sorts :
+  ∀ l, sorted (sort_monomials l).
+Proof.
+  remember (λ (_ : list pterm) ls, LocallySorted pterm_le ls) as P.
+  pose proof (sort_monomials_ind P); subst P; apply H; clear H;
+  try now (intros; constructor).
+  intros l la Heq Hc2 l1 l2 Hsplit Hsort1 Hsort2.
+  apply mergesort_monomials_sorted; auto.
+Qed.
+
+Theorem reduce_monomials_correct :
+  ∀ l, l ≡ₗ (reduce_monomials l).
+Proof.
+  apply reduce_monomials_ind; simpl; auto.
+  - intros l z v Hl HEq st.
+    apply Z.eqb_eq in HEq; subst.
+    apply fold_left_mul_0.
+  - intros l z1 v1 z2 v2 l' Hl HEq Heqv st.
+    rewrite <- Heqv; simpl.
+    pose proof (cmp_vars_eq_iff _ _ HEq); subst.
+    rewrite <- Z.add_assoc. f_equal.
+    apply vars_pow_add.
+  - intros l z1 v1 z2 v2 l' Hl cmp_res HEq Hcmp Hnz Heqv st; simpl.
+    pose proof (reflect_iff _ _ (Z.eqb_spec z1 0)) as Hreflect.
+    apply Hreflect in Hnz; subst z1.
+    rewrite fold_left_mul_0.
+    rewrite <- Heqv; simpl; lia.
+  - intros l z1 v1 z2 v2 l' Hl cmp_res HEq Hcmp Hnz Heqv st; simpl.
+    rewrite <- Heqv; auto.
+Qed.
+
+Theorem reduce_monomials_sort_preserve :
+  ∀ l, sorted l → sorted (reduce_monomials l).
+Proof.
+  strong_list_induction.
+  intros n' IH l Hlen Hsort.
+  destruct l as [| [c1 v1] l'] eqn:?; auto;
+  destruct l' as [| [c2 v2] l''] eqn:?; auto;
+  rewrite reduce_monomials_equation;
+  [ destruct (Z.eqb_spec c1 0); auto; constructor |].
+  destruct (cmp_vars v1 v2) eqn:?; [| destruct (Z.eqb_spec c1 0) |].
+  - simpl in *.
+    apply (IH (1+List.length l'')); try (subst; simpl; lia).
+    inv Hsort.
+    apply Sorted_LocallySorted_iff, Sorted_inv in H1.
+    destruct H1.
+    apply Sorted_LocallySorted_iff, Sorted_cons; auto.
+    pose proof (cmp_vars_eq_iff _ _ Heqc); subst.
+    eapply HdRel_pterm_le_const_invariant, H0.
+  - inv Hsort.
+    apply (IH (1+List.length l'')); auto;
+      try (subst; simpl; lia).
+  - apply Sorted_LocallySorted_iff, Sorted_cons.
+    + simpl in *. inv Hsort.
+      apply Sorted_LocallySorted_iff, (IH (1+List.length l'')); auto;
+      subst; simpl; lia.
+    + apply reduce_monomials_HdRel_pterm_le; auto.
+  - inversion Hsort.
+    unfold pterm_le in H3; simpl in H3.
+    exfalso; apply H3, Heqc.
+Qed.
+
+Lemma reduce_clears_zeros :
+  ∀ l, reduce_monomials l = [] → Forall (λ '(PTerm c _), c = 0%Z) l.
+Admitted.
+
+Lemma reduce_monom_not_rep1 :
+  ∀ l' c1 c2 v1 v2 l1, cmp_vars v1 v2 = Lt →
+  sorted (PTerm c1 v1 :: PTerm c2 v2 :: l') →
+  PTerm c1 v1 :: l1 = PTerm c1 v1 :: reduce_monomials (PTerm c2 v2 :: l') →
+  (∃ c3 v3 l2, l1 = PTerm c3 v3 :: l2 /\ cmp_vars v1 v3 = Lt) \/
+    fold_left Z.add (map const (PTerm c2 v2 :: l')) 0%Z = 0%Z /\
+    reduce_monomials (PTerm c2 v2 :: l') = [].
+Proof.
+  strong_list1_induction.
+  intros n' IH l' Hlen c1 c2 v1 v2 l1 HLt Hsort Heq.
+  destruct l' as [| [c3 v3] l''];
+  [ rewrite reduce_monomials_equation in *; destruct (Z.eqb_spec c2 0);
+    [ right; auto |] |];
+  [ left; destruct l1; [ inv Heq; apply cmp_vars_refl_nlt in Heqc; contradiction |];
+    inv Heq; repeat eexists; auto |].
+  rewrite reduce_monomials_equation in Heq.
+  destruct (cmp_vars v2 v3) eqn:?; [| destruct (Z.eqb_spec c2 0) |].
+  - simpl in Hlen.
+    edestruct (IH (List.length l'')) as [[c4 [v4 [l4 [Hsplit Hcmp]]]] | [Heqz Hl'nil]];
+    try (subst; simpl; lia);
+    [ reflexivity | apply HLt | | apply Heq | left; repeat eexists; eauto
+    | right; rewrite reduce_monomials_equation, Heqc; split; auto ].
+    pose proof (cmp_vars_eq_iff _ _ Heqc); subst v2.
+    eapply sorted_const_invariant, sorted_shadow, Hsort.
+  - pose proof (cmp_vars_trans _ _ _ HLt Heqc).
+    edestruct (IH (List.length l'')) as [[c4 [v4 [l4 [Hsplit Hcmp]]]]|[Heqz Hl'nil]];
+    try (subst; simpl; lia);
+    [ reflexivity | apply H | | apply Heq | left; repeat eexists; eauto
+    | right; rewrite reduce_monomials_equation, Heqc; split; auto ].
+    + eapply sorted_const_invariant, sorted_shadow, Hsort.
+    + apply reduce_clears_zeros in Hl'nil. inv Hl'nil.
+      rewrite map_spec, fold_left_spec.
+      replace (0+_)%Z with 0%Z by (simpl; lia); auto.
+    + apply Z.eqb_eq in e; now rewrite e.
+  - inversion Heq. destruct l1; inversion H0; subst p. simpl in Hlen.
+    edestruct (IH (List.length l'')) as [[c4 [v4 [l4 [Hsplit Hcmp]]]]|[Heqz Hl'nil]];
+    try (subst; simpl; lia);
+    [ reflexivity | apply Heqc | | apply H0 | left; repeat eexists; eauto
+    | left; repeat eexists; eauto ].
+    inv Hsort; auto.
+  - inv Hsort; inv H1. unfold pterm_le in H5; simpl in H5.
+    exfalso. apply H5, Heqc.
+Qed.
+
+Lemma reduce_monomials_not_rep :
+  ∀ l l' a, sorted l → a :: l' = reduce_monomials l →
+    ~In a l'.
+Proof.
+  strong_list1_induction.
+  intros n' IH l Hlen l' a Hsort Heq.
+  intro HIn.
+  edestruct (in_split _ _ HIn) as [l1 [l2 Hsplit]].
+  subst l'.
+  pose proof (reduce_monomials_sort_preserve _ Hsort).
+  rewrite reduce_monomials_equation in Heq.
+  destruct l as [| [c1 v1] [| [c2 v2] l']] eqn:?;
+  [ inv Heq
+  | destruct (Z.eqb_spec c1 0); [ inv Heq | inv Heq; destruct l1; inv H2 ] |].
+  destruct (cmp_vars v1 v2) eqn:?; [| destruct (Z.eqb_spec c1 0) |].
+  - assert (~In a (l1++a::l2)). {
+      simpl in Hlen.
+      (* inversion Hsort; clear Hsort. *)
+      eapply (IH (1+List.length l')); try (subst; simpl; lia);
+      [| | apply Heq ]; simpl; try lia.
+      apply Sorted_LocallySorted_iff, Sorted_inv in Hsort; destruct Hsort.
+      apply Sorted_inv in H0; destruct H0.
+      apply Sorted_LocallySorted_iff, Sorted_cons; auto.
+      destruct l' as [| [c3 v3] l']; constructor.
+      pose proof (cmp_vars_eq_iff _ _ Heqc); subst v2.
+      inv H2.
+      unfold pterm_le in *; now simpl in *.
+    }
+    apply H0, HIn.
+  - simpl in Hlen.
+    eapply (IH (1+List.length l')); try (subst; simpl; lia);
+    [| inv Hsort | apply Heq | ]; eauto; simpl; lia.
+  - apply Z.eqb_neq in n.
+    inversion Heq; subst a.
+    rewrite reduce_monomials_equation, Heqc, n in H.
+    remember H as HContra; clear HeqHContra; rewrite <- H2 in HContra.
+    destruct (reduce_monom_not_rep1 _ _ _ _ _ _ Heqc Hsort Heq)
+      as [[c3 [v3 [l'' [Hsplit Hcmp]]]]|[Heqz Hl'nil]].
+    + destruct l1; inversion Hsplit;
+        [ subst; apply cmp_vars_refl_nlt in Hcmp; contradiction |].
+      subst p.
+      apply Sorted_LocallySorted_iff, Sorted_StronglySorted in HContra;
+      [| apply Rel1_Transitive_pterm_le ].
+      simpl in HContra.
+      inv HContra; inv H4.
+      apply Forall_app in H6; destruct H6 as [? ?].
+      inv H1; unfold pterm_le in H7; simpl in H7.
+      apply H7. now rewrite cmp_vars_antisym, Hcmp.
+    + rewrite Hl'nil in H2. destruct l1; inv H2.
+  - inv Hsort. unfold pterm_le in H4; simpl in H4.
+    apply H4, Heqc.
+Qed.
+
+Theorem reduce_monomials_canonical :
+  ∀ l, sorted l → canon_pterm (reduce_monomials l).
+Proof.
+  strong_list_induction.
+  intros n' IH l Hlen Hsort.
+  destruct l as [| [c1 v1] l'] eqn:?; auto;
+  destruct l' as [| [c2 v2] l''] eqn:?; auto;
+  [ rewrite reduce_monomials_equation; simpl;
+    destruct (Z.eqb_spec c1 0); [ auto | apply canon_pterm_single ] |].
+  rewrite reduce_monomials_equation.
+  destruct (cmp_vars v1 v2) eqn:?; [| destruct (Z.eqb_spec c1 0) |].
+  - simpl in *.
+    apply (IH (1+List.length l'')); try (subst; simpl; lia).
+    inv Hsort.
+    apply Sorted_LocallySorted_iff, Sorted_inv in H1.
+    destruct H1.
+    apply Sorted_LocallySorted_iff, Sorted_cons; auto.
+    pose proof (cmp_vars_eq_iff _ _ Heqc); subst.
+    eapply HdRel_pterm_le_const_invariant, H0.
+  - inv Hsort.
+    apply (IH (1+List.length l'')); auto; subst; simpl; lia.
+  - apply Z.eqb_neq in n.
+    apply canon_pterm_cons.
+    + eapply reduce_monomials_not_rep; [ eassumption |].
+      symmetry; now rewrite reduce_monomials_equation, Heqc, n.
+    + simpl in *.
+      apply (IH (1+List.length l'')); try (subst; simpl; lia).
+      inv Hsort; assumption.
+  - inv Hsort. unfold pterm_le in H3; simpl in H3.
+    exfalso; apply H3, Heqc.
+Qed.
+
+Theorem reduce_monomials_non_zero_const :
+  ∀ l, sorted l → non_zero_const (reduce_monomials l).
+Proof.
+  strong_list_induction.
+  intros n' IH l Hlen Hsort.
+  destruct l as [| [c1 v1] l'] eqn:?; auto;
+  destruct l' as [| [c2 v2] l''] eqn:?; rewrite reduce_monomials_equation;
+    [ destruct (Z.eqb_spec c1 0) |]; auto.
+  destruct (cmp_vars v1 v2) eqn:?; [| destruct (Z.eqb_spec c1 0) |].
+  - simpl in *.
+    apply (IH (1+List.length l'')); try (subst; simpl; lia).
+    inv Hsort.
+    apply Sorted_LocallySorted_iff, Sorted_inv in H1.
+    destruct H1.
+    apply Sorted_LocallySorted_iff, Sorted_cons; auto.
+    pose proof (cmp_vars_eq_iff _ _ Heqc); subst.
+    eapply HdRel_pterm_le_const_invariant, H0.
+  - inv Hsort.
+    apply (IH (1+List.length l'')); auto; subst; simpl; lia.
+  - constructor; auto.
+    inv Hsort.
+    apply (IH (1+List.length l'')); auto; subst; simpl; lia.
+  - inv Hsort. unfold pterm_le in H3; simpl in H3.
+    exfalso; apply H3, Heqc.
+Qed.
+
+  
 
